src/FrameStack/Scoping.v
@@ -1,147 +1,152 @@
-Require Export ExpSyntax.
+From CoreErlang Require Export Syntax.
+Import ListNotations.
 
-Fixpoint patternScope (p : Pattern) : nat :=
+Fixpoint PatScope (p : Pat) : nat :=
 match p with
  (*| PVar v => 1*)
  | PVar   => 1
  | PLit l => 0
- | PCons hd tl => patternScope hd + patternScope tl
- | PTuple l => fold_right (fun x y => (patternScope x) + y) 0 l
- | PMap l => fold_right (fun '(a,b) y => (patternScope a) + (patternScope b) + y) 0 l
+ | PCons hd tl => PatScope hd + PatScope tl
+ | PTuple l => fold_right (fun x y => (PatScope x) + y) 0 l
+ | PMap l => fold_right (fun '(a,b) y => (PatScope a) + (PatScope b) + y) 0 l
  | PNil => 0
-end
-.
+end.
 
-Definition patternListScope (pl : list Pattern) : nat :=
-fold_right (fun x y => (patternScope x) + y) 0 pl
-.
+Definition PatListScope (pl : list Pat) : nat :=
+  fold_right (fun x y => (PatScope x) + y) 0 pl.
+
+Reserved  Notation "'NVAL' Γ ⊢ e" (at level 69, no associativity).
+Reserved Notation "'VAL' Γ ⊢ v" (at level 69, no associativity).
+Reserved Notation "'EXP' Γ ⊢ e" (at level 69, no associativity).
+
+Open Scope program_scope.
 
 (** For language elements involving lists (e.g. tuples) we originally used Forall in the constructors (which lead to nested induction), this was easier to read, but Coq can not generate strong enough induction hypothesises for proofs, so we ended up using indexing witch is a bit harder to read in the definition, but Coq can use it to generate the needed hypothesises. *)
-Inductive ExpScoped : Expression -> nat -> Prop :=
-| scoped_val (v : ValueExpression) (n : nat)    : ValExpScoped v n    -> ExpScoped (Val v) n
-| scoped_exp (e : NonValueExpression) (n : nat) : NonValExpScoped e n -> ExpScoped (Exp e) n
+Inductive ExpScoped : nat -> Exp -> Prop :=
+| scoped_val (v : Val) (Γ : nat):
+  VAL Γ ⊢ v -> EXP Γ ⊢ (VVal v)
 
-with ValExpScoped : ValueExpression -> nat -> Prop :=
-| scoped_nil (n : nat)                                : ValExpScoped VNil n
-| scoped_lit (l : Literal) (n : nat)                  : ValExpScoped (VLit l) n
-| scoped_var (v : nat) (n : nat)                      : n > v -> ValExpScoped (VVar v) n
-| scoped_funId (fi : nat) (n : nat)                   : n > fi -> ValExpScoped (VFunId fi) n
-(*| scoped_vtuple (l : list ValueExpression) (n : nat)  : Forall (fun x => ValExpScoped x n) l -> ValExpScoped (VTuple l) (n) *)
-| scoped_vtuple (l : list ValueExpression) (n : nat)  : (forall i, i < length l -> ValExpScoped (nth i l VNil) n) -> ValExpScoped (VTuple l) (n)
-| scoped_vcons (hd tl : ValueExpression) (n : nat)    : ValExpScoped hd n -> ValExpScoped tl n -> ValExpScoped (VCons hd tl) (n)
-(*| scoped_vmap (l : list (ValueExpression * ValueExpression)) (n : nat) : 
-  Forall (fun x => ValExpScoped x n) (map (fun '(x,y) => x) l) ->
-  Forall (fun x => ValExpScoped x n) (map (fun '(x,y) => y) l)
-  -> ValExpScoped (VMap l) n*)
-(*| scoped_vmap (l : list (ValueExpression * ValueExpression)) (n : nat) : (* This is the previous definition, in the newer we create a Exp List first. *)
-  (forall i, i< length l -> ValExpScoped (fst (nth i l (VNil,VNil))) n) ->
-  (forall i, i< length l -> ValExpScoped (snd (nth i l (VNil,VNil))) n)
-  -> ValExpScoped (VMap l) n*)
-| scoped_vmap (l : list (ValueExpression * ValueExpression)) (n : nat) : 
-  (forall i, i< length l -> ValExpScoped (nth i (map fst l) VNil) n) ->
-  (forall i, i< length l -> ValExpScoped (nth i (map snd l) VNil) n)
-  -> ValExpScoped (VMap l) n
-(*| scoped_vvalues (el : list ValueExpression) (n : nat)   : Forall (fun x => ValExpScoped x n) el -> ValExpScoped (VValues el) (n)*)
-(*| scoped_vvalues (el : list ValueExpression) (n : nat)   : (forall i, i < length el -> ValExpScoped (nth i el VNil) n) -> ValExpScoped (VValues el) (n) *)
-(*| scoped_vclos (ext : list (nat * nat * Expression)) (id : nat) (vl : nat) (e : Expression) (n m : nat) :
-  Forall (fun x => x <= m) (map (fun '(a,b,x) => b) ext) ->
-  Forall (fun x => ExpScoped x (m + length ext)) (map (fun '(a,b,x) => x) ext) ->
-  ExpScoped e (vl + length ext) ->
-  ValExpScoped (VClos ext id vl e) n*)
-(*| scoped_vclos (ext : list (nat * nat * Expression)) (id : nat) (vl : nat) (e : Expression) (n m : nat) :
-  (* This is the previous definition, in the newer we create a Exp List first. *)
-  (forall i, i < length ext -> ExpScoped (snd (nth i ext (0,0,Val VNil))) (length ext + (snd(fst (nth i ext (0,0,Val VNil)))) + n) ) ->
-  ExpScoped e (length ext + vl + n) ->
-  ValExpScoped (VClos ext id vl e) n *)
-| scoped_vclos (ext : list (nat * nat * Expression)) (id : nat) (vl : nat) (e : Expression) (n : nat) :
-  (forall i, i < length ext -> ExpScoped (nth i (map snd ext) (Val VNil)) (length ext + (nth i (map snd (map fst ext)) 0) + n) ) ->
-  ExpScoped e (length ext + vl + n) ->
-  ValExpScoped (VClos ext id vl e) n
+| scoped_exp (e : NonVal) (Γ : nat):
+  NVAL Γ ⊢ e -> EXP Γ ⊢ (EExp e)
 
-with NonValExpScoped : NonValueExpression -> nat -> Prop :=
-| scoped_efun (vl : nat) (e : Expression) (n : nat)  : ExpScoped e (vl + n) -> NonValExpScoped (EFun vl e) (n)
-(* | scoped_etuple (l : list Expression) (n : nat) : Forall (fun x => ExpScoped x n) l -> NonValExpScoped (ETuple l) (n)) *)
-| scoped_etuple (l : list Expression) (n : nat) : (forall i, i < length l -> ExpScoped (nth i l (Val VNil)) n) -> NonValExpScoped (ETuple l) (n)
-| scoped_econs (hd tl : Expression) (n : nat)   : ExpScoped hd n -> ExpScoped tl n -> NonValExpScoped (ECons hd tl) (n)
-(*| scoped_emap (l : list (Expression * Expression)) (n : nat) : 
-  Forall (fun x => ExpScoped x n) (map (fun '(x,y) => x) l) ->
-  Forall (fun x => ExpScoped x n) (map (fun '(x,y) => y) l)
-  -> NonValExpScoped (EMap l) n *)
-(*| scoped_emap (l : list (Expression * Expression)) (n : nat) : (* This is the previous definition, in the newer we create a Exp List first. *)
-  (forall i, i< length l -> ExpScoped (fst (nth i l (Val VNil,Val VNil))) n) ->
-  (forall i, i< length l -> ExpScoped (snd (nth i l (Val VNil,Val VNil))) n)
-  -> NonValExpScoped (EMap l) n *)
-| scoped_emap (l : list (Expression * Expression)) (n : nat) : 
-  (forall i, i< length l -> ExpScoped (nth i (map fst l) (Val VNil)) n) ->
-  (forall i, i< length l -> ExpScoped (nth i (map snd l) (Val VNil)) n)
-  -> NonValExpScoped (EMap l) n
-(* | scoped_evalues (el : list Expression) (n : nat)   : Forall (fun x => ExpScoped x n) el -> NonValExpScoped (EValues el) (n) *)
-| scoped_evalues (el : list Expression) (n : nat)   : (forall i, i < length el -> ExpScoped (nth i el (Val VNil)) n) -> NonValExpScoped (EValues el) (n)
-(*| scoped_call (f : string) (l : list Expression) (n : nat)      : Forall (fun x => ExpScoped x n) l -> NonValExpScoped (ECall f l) (n) *)
-| scoped_call (f : string) (l : list Expression) (n : nat)      : (forall i, i < length l -> ExpScoped (nth i l (Val VNil)) n) -> NonValExpScoped (ECall f l) (n)
-(* | scoped_primOp (f : string) (l : list Expression) (n : nat)    : Forall (fun x => ExpScoped x n) l -> NonValExpScoped (EPrimOp f l) (n) *)
-| scoped_primOp (f : string) (l : list Expression) (n : nat)    : (forall i, i < length l -> ExpScoped (nth i l (Val VNil)) n) -> NonValExpScoped (EPrimOp f l) (n)
-(* | scoped_app (exp: Expression) (l : list Expression) (n : nat)  : ExpScoped exp n -> Forall (fun x => ExpScoped x n) l -> NonValExpScoped (EApp exp l) (n) *)
-| scoped_app (exp: Expression) (l : list Expression) (n : nat)  : ExpScoped exp n -> (forall i, i < length l -> ExpScoped (nth i l (Val VNil)) n) -> NonValExpScoped (EApp exp l) (n)
-(* | scoped_case (e : Expression) (l : list ((list Pattern) * Expression * Expression)) (m n : nat) : 
-  ExpScoped e n -> 
-  Forall (fun x => patternListScope x <= m) (map (fun '(x,y,z) => x) l) ->
-  Forall (fun x => ExpScoped x (m+n))       (map (fun '(x,y,z) => y) l) ->
-  Forall (fun x => ExpScoped x (m+n))       (map (fun '(x,y,z) => z) l)
-  -> NonValExpScoped (ECase e l) (n) *)
-(*| scoped_case (e : Expression) (l : list ((list Pattern) * Expression * Expression)) (n : nat) : (* This is the previous definition, in the newer we create a Exp List first. *)
-  ExpScoped e n -> 
-  (forall i, i< length l -> ExpScoped (snd(fst(nth i l (nil, Val VNil, Val VNil)))) ((patternListScope (fst(fst(nth i l (nil, Val VNil, Val VNil))))) + n)) ->
-  (forall i, i< length l -> ExpScoped (snd(nth i l (nil, Val VNil, Val VNil))) ((patternListScope (fst(fst(nth i l (nil, Val VNil, Val VNil))))) + n))
-  -> NonValExpScoped (ECase e l) (n) *)
-| scoped_case (e : Expression) (l : list ((list Pattern) * Expression * Expression)) (n : nat) : 
-  ExpScoped e n -> 
-  (forall i, i< length l -> ExpScoped (nth i (map snd (map fst l)) (Val VNil)) ((patternListScope (nth i (map fst (map fst l)) nil)) + n)) ->
-  (forall i, i< length l -> ExpScoped (nth i (map snd l) (Val VNil))           ((patternListScope (nth i (map fst (map fst l)) nil)) + n))
-  -> NonValExpScoped (ECase e l) (n)
-| scoped_let (l : nat) (e1 e2 : Expression) (n : nat) : 
-  ExpScoped e1 n -> ExpScoped e2 (l+n)
-  -> NonValExpScoped (ELet l e1 e2) n
-| scoped_seq (e1 e2 : Expression) (n : nat) : ExpScoped e1 n -> ExpScoped e2 n -> NonValExpScoped (ESeq e1 e2) n
+where "'EXP' Γ ⊢ e" := (ExpScoped Γ e)
 
-(*| scoped_letRec (l : list (nat * Expression)) (e : Expression) (m n : nat) :
-  Forall (fun x => x <= m) (map (fun '(x,y) => x) l) ->
-  Forall (fun x => ExpScoped x (S(m) + n)) (map (fun '(x,y) => y) l) ->
-  (*in m + n we may need +(length l) as well because of function definitions in letRec *)
-  ExpScoped e (n + (length l))
-  -> NonValExpScoped (ELetRec l e) n *)
+with ValScoped : nat -> Val -> Prop :=
+| scoped_nil (n : nat): VAL n ⊢ VNil
+
+| scoped_lit (l : Lit) (n : nat): VAL n ⊢ (VLit l)
+
+| scoped_var (v : Var) (n : nat): n > v -> VAL n ⊢ (VVar v)
+
+| scoped_funId (fi : FunId) (n : nat): n > fst fi -> VAL n ⊢ (VFunId fi)
+
+| scoped_vtuple (l : list Val) (n : nat):
+  (forall i, i < length l -> VAL n ⊢ (nth i l VNil))
+-> 
+  VAL n ⊢ (VTuple l)
+| scoped_vcons (hd tl : Val) (n : nat):
+  VAL n ⊢ hd -> VAL n ⊢ tl
+->
+  VAL n ⊢ (VCons hd tl)
+
+| scoped_vmap (l : list (Val * Val)) (n : nat) : 
+  (forall i, i < length l -> VAL n ⊢ (nth i (map fst l) VNil)) ->
+  (forall i, i < length l -> VAL n ⊢ (nth i (map snd l) VNil))
+  ->
+  VAL n ⊢ (VMap l)
+
+| scoped_vclos (ext : list (nat * nat * Exp)) (id : nat) (vl : nat) (e : Exp) (n : nat) :
+  (forall i, i < length ext ->
+  EXP (length ext + (nth i (map (snd ∘ fst) ext) 0) + n) ⊢ 
+      (nth i (map snd ext) (VVal VNil))) ->
+  EXP (length ext + vl + n) ⊢ e->
+  VAL n ⊢ (VClos ext id vl e)
+where "'VAL' Γ ⊢ e" := (ValScoped Γ e)
+
+with NonValScoped : nat -> NonVal -> Prop :=
+| scoped_efun (vl : nat) (e : Exp) (n : nat):
+  EXP vl + n ⊢ e -> NVAL n ⊢ EFun vl e
+
+| scoped_etuple (l : list Exp) (n : nat) :
+  (forall i, i < length l -> EXP n ⊢ (nth i l (VVal VNil)))
+->
+  NVAL n ⊢ (ETuple l)
+
+| scoped_econs (hd tl : Exp) (n : nat):
+  EXP n ⊢ hd -> EXP n ⊢ tl
+->
+  NVAL n ⊢ (ECons hd tl)
+
+| scoped_emap (l : list (Exp * Exp)) (n : nat): 
+  (forall i, i< length l -> EXP n ⊢ (nth i (map fst l) (VVal VNil))) ->
+  (forall i, i< length l -> EXP n ⊢ (nth i (map snd l) (VVal VNil)))
+->
+  NVAL n ⊢ (EMap l)
+
+| scoped_evalues (el : list Exp) (n : nat):
+  (forall i, i < length el -> EXP n ⊢ (nth i el (VVal VNil)))
+->
+  NVAL n ⊢ (EValues el)
+
+| scoped_call (f : string) (l : list Exp) (n : nat):
+  (forall i, i < length l -> EXP n ⊢ (nth i l (VVal VNil)))
+->
+  NVAL n ⊢ (ECall f l)
+
+| scoped_primOp (f : string) (l : list Exp) (n : nat):
+  (forall i, i < length l -> EXP n ⊢ (nth i l (VVal VNil)))
+->
+  NVAL n ⊢ (EPrimOp f l)
+
+| scoped_app (exp: Exp) (l : list Exp) (n : nat)  :
+  EXP n ⊢ exp ->
+  (forall i, i < length l -> EXP n ⊢ (nth i l (VVal VNil)))
+->
+  NVAL n ⊢ (EApp exp l)
+
+| scoped_case (e : Exp) (l : list ((list Pat) * Exp * Exp)) (n : nat) : 
+  EXP n ⊢ e ->
+  (* todo:  *)
+  (forall i, i < length l ->
+    EXP (PatListScope (nth i (map (fst ∘ fst) l) [])) + n ⊢
+        nth i (map (snd ∘ fst) l) (VVal VNil)) ->
+  (forall i, i < length l ->
+    EXP (PatListScope (nth i (map (fst ∘ fst) l) [])) + n ⊢
+        (nth i (map snd l) (VVal VNil)))
+->
+  NVAL n ⊢ (ECase e l)
+
+  | scoped_let (l : nat) (e1 e2 : Exp) (n : nat) : 
+  EXP n ⊢ e1 -> EXP l + n ⊢ e2
+->
+  NVAL n ⊢ (ELet l e1 e2)
+
+| scoped_seq (e1 e2 : Exp) (n : nat) :
+  EXP n ⊢ e1 -> EXP n ⊢ e2
+->
+  NVAL n ⊢ (ESeq e1 e2)
   
-(* | scoped_letRec (l : list (nat * Expression)) (e : Expression) (n : nat) : (* This is the previous definition, in the newer we create a Exp List first. *)
-  (forall i, i < length l -> ExpScoped (snd(nth i l (0,Val VNil))) ((length l) + (fst(nth i l (0,Val VNil))) + n)) ->
-  ExpScoped e ((length l) + n)
-  -> NonValExpScoped (ELetRec l e) n *)
+| scoped_letRec (l : list (nat * Exp)) (e : Exp) (n : nat) :
+  (forall i, i < length l ->
+    EXP (length l) + (nth i (map fst l) 0) + n ⊢ 
+        nth i (map snd l) (VVal VNil)) ->
+  EXP (length l) + n ⊢ e
+->
+  NVAL n ⊢ (ELetRec l e)
   
-| scoped_letRec (l : list (nat * Expression)) (e : Expression) (n : nat) :
-  (forall i, i < length l -> ExpScoped (nth i (map snd l) (Val VNil)) ((length l) + (nth i (map fst l) 0) + n)) ->
-  ExpScoped e ((length l) + n)
-  -> NonValExpScoped (ELetRec l e) n
-  
-| scoped_try (e1 : Expression) (vl1 : nat) (e2 : Expression) (vl2 : nat) (e3 : Expression) (n : nat) : 
-  ExpScoped e1 n -> 
-  ExpScoped e2 (vl1 + n) ->
-  ExpScoped e3 (vl2 + n)
-  -> NonValExpScoped (ETry e1 vl1 e2 vl2 e3) n
-.
-
-Notation "'NVAL' Γ ⊢ e" := (NonValExpScoped e Γ)
-         (at level 69, no associativity).
-Notation "'VAL' Γ ⊢ v" := (ValExpScoped v Γ)
-         (at level 69, no associativity).
-Notation "'EXP' Γ ⊢ e" := (ExpScoped e Γ)
-         (at level 69, no associativity).
+| scoped_try (e1 : Exp) (vl1 : nat) (e2 : Exp) (vl2 : nat) (e3 : Exp) (n : nat) : 
+  EXP n ⊢ e1 -> 
+  EXP vl1 + n ⊢  e2 ->
+  EXP vl2 + n ⊢  e3 
+->
+  NVAL n ⊢ (ETry e1 vl1 e2 vl2 e3)
+where "'NVAL' Γ ⊢ e" := (NonValScoped Γ e).
 
 Notation "'EXPCLOSED' e"    := (EXP 0 ⊢ e) (at level 5).
 Notation "'VALCLOSED' v"    := (VAL 0 ⊢ v) (at level 5).
 Notation "'NONVALCLOSED' v" := (NVAL 0 ⊢ v) (at level 5).
 
 Scheme ExpScoped_ind2     := Induction for ExpScoped Sort Prop
-  with ValScoped_ind2     := Induction for ValExpScoped Sort Prop
-  with NonValScoped_ind2  := Induction for NonValExpScoped Sort Prop.
+  with ValScoped_ind2     := Induction for ValScoped Sort Prop
+  with NonValScoped_ind2  := Induction for NonValScoped Sort Prop.
 Combined Scheme scoped_ind from ExpScoped_ind2, ValScoped_ind2, NonValScoped_ind2.
-
-Check scoped_ind.
